oopsla16/dot_soundness_alt.v
@@ -11,12 +11,18 @@ Inductive vtp(*possible types*) : nat(*pack count*) -> venv -> id -> ty -> nat(*
     stp [] G1 T1 TX n1 ->
     stp [] G1 TX T2 n2 ->
     vtp m G1 x (TMem l T1 T2) (S (n1+n2))
-| vtp_fun: forall m G1 x l ds dsx T1 T2 T3 T4 T2' T4' t T1x T2x tx T' T2x' n1 n2 n3 n4,
+| vtp_fun: forall m G1 x l ds dsx OT1 OT2 OT1x OT2x T1 T2 T3 T4 T2' T4' t T1x T2x tx T' T2x' n1 n2 n3 n4,
     index x G1 = Some (vobj ds) ->
-    index l (dms_to_list ds) = Some (dfun T1 T2 t) ->
+    index l (dms_to_list ds) = Some (dfun OT1 OT2 t) ->
+    eq_some OT1 T1 ->
+    eq_some OT2 T2 ->
     subst_dms x dsx = ds ->
     dms_has_type [T'] G1 dsx T' n4 ->
-    subst_dm x (dfun T1x T2x tx) = (dfun T1 T2 t) ->
+    subst_dm x (dfun OT1x OT2x tx) = (dfun OT1 OT2 t) ->
+    eq_some OT1x T1x ->
+    eq_some OT2x T2x ->
+    substt x T1x = T1 ->
+    substt x T2x = T2 ->
     T2x' = (open 0 (TVar false 1) T2x) ->
     has_type [T1x;T'] G1 tx T2x' n3 ->
     stp [] G1 T3 T1 n1 ->
@@ -76,8 +82,8 @@ Proof.
   (* vtp *)
   - econstructor. simpl. eauto.
   - econstructor. eapply index_extend. eauto. eauto. eapply stp_extend. eauto. eapply stp_extend. eauto.
-  - econstructor. eapply index_extend. eauto. eauto. eauto.
-    eapply dms_has_type_extend. eauto. eauto. eauto.
+  - econstructor. eapply index_extend. eauto. eauto. eauto. eauto. eauto.
+    eapply dms_has_type_extend. eauto. eauto. eauto. eauto. eauto. eauto. eauto.
     eapply has_type_extend. eauto. eapply stp_extend. eauto. eauto. eauto.
     eapply closed_extend. eauto. eapply closed_extend. eauto. eapply stp_extend. eauto.
   - econstructor. eapply IHn. eauto. omega. eapply closed_extend. eauto.
@@ -417,17 +423,19 @@ Proof.
   - Case "fun". inversion H0; subst; invty.
     + SCase "top". repeat eexists. eapply vtp_top. eapply index_max. eauto. eauto.
     + SCase "fun". invty. subst.
+      remember (substt x T2x) as T0.
       assert (stpd [T8] G1 (open 0 (TVar false 0) T0) (open 0 (TVar false 0) T5)) as A. {
         eapply stp_narrow_norec. simpl. eassumption. simpl. eassumption.
       }
       destruct A as [na A].
       repeat eexists. eapply vtp_fun. eauto. eauto. eauto. eauto. eauto. eauto. eauto.
+      eauto. eauto. eauto. eauto. eauto. eauto.
       eapply stp_trans. eauto. eauto. eauto. eauto. eauto. eauto. eauto. reflexivity.
     + SCase "sel2".
       assert (vtpdd m1 G1 x TX). eapply IHn; eauto. omega.
       euv. repeat eexists. eapply vtp_sel. eauto. eauto. eauto. eauto.
     + SCase "sel2".
-      eapply stp_closed2 in H0. simpl in H0. inversion H0. subst. inversion H17. omega.
+      eapply stp_closed2 in H0. simpl in H0. inversion H0. subst. inversion H18. omega.
     + SCase "and".
       assert (vtpdd m1 G1 x T6). eapply IHn; eauto. omega. euv.
       assert (vtpdd m1 G1 x T7). eapply IHn; eauto. omega. euv.
@@ -672,10 +680,10 @@ Proof.
     }
     assert (closed 0 (length G1) 0 (substt x T11)) as HC11. {
       unfold substt in *. simpl in HC. inversion HC; subst.
-      inversion H8; subst. eauto.
+      inversion H10; subst. eauto.
     }
     assert (closed 1 (length G1) 0 (open 0 (TVar false 0) (substt x T12))) as HC12. {
-      unfold substt in *. simpl in HC. inversion HC; subst. inversion H8; subst.
+      unfold substt in *. simpl in HC. inversion HC; subst. inversion H10; subst.
       eapply closed_open. eapply closed_upgrade_gh. eauto. omega.
       econstructor. omega.
     }
@@ -689,11 +697,13 @@ Proof.
     eu.
     destruct Hds as [dsa Hdsa]. simpl in Hdsa.
     edestruct IHdms_has_type as [? [? AS]]. eauto. eauto. eauto.
-    exists (dsa ++ [dfun T11 T12 t12]). rewrite <- app_assoc. simpl. eauto. eauto. eauto.
+    exists (dsa ++ [dfun OT11 OT12 t12]). rewrite <- app_assoc. simpl. eauto. eauto. eauto.
     unfold substt in *. simpl.
     repeat eexists. eapply vtp_and. eapply vtp_fun. eauto.
-    erewrite index_subst_dms with (D:=dfun T11 T12 t12). simpl. reflexivity. eauto.
+    erewrite index_subst_dms with (D:=dfun OT11 OT12 t12). simpl. reflexivity. eauto.
+    eapply subst_eq_some; eauto. eapply subst_eq_some; eauto.
     eauto. eapply HT0. simpl. reflexivity. eauto. eauto. eauto. eauto. eauto.
+    eauto. eauto. eauto. eauto.
     eapply closed_subst. eauto. econstructor. eapply index_max. eauto.
     eapply closed_subst. eauto. econstructor. eapply index_max. eauto.
     eauto. eauto. eauto. eauto.
@@ -888,6 +898,7 @@ Proof.
     rewrite app_length in H6. simpl in H6. eauto.
     eapply has_type_closed1. eauto. eauto.
     unfold substt. simpl. rewrite <- length_subst_dms. reflexivity.
+    eapply subst_eq_some; eauto. eapply subst_eq_some; eauto.
 Grab Existential Variables.
 apply 0. apply 0.
 Qed.
@@ -953,32 +964,33 @@ Proof.
         assert (exists m n1, vtp m G1 x (TFun l T1 T) n1). eapply hastp_inv. eauto.
         assert (exists m n1, vtp m G1 x0 T1 n1). eapply hastp_inv. eauto.
         ev. inversion H2. subst.
+        remember (substt x T1x) as T0. remember (substt x T2x) as T2.
         assert (vtpdd x1 G1 x0 T0). eapply vtp_widen. eauto. eauto. eauto. eauto. eauto.
         euv.
         assert (exists T, (exists n1, has_type [] G1 (tvar true x) T n1) /\ substt x T' = T) as A. {
           eexists. split. eexists. eapply T_Vary. eauto. eauto. eauto. eauto.
-          eapply closed_subst. eapply dms_has_type_closed in H10. eauto. econstructor.
+          eapply closed_subst. eapply dms_has_type_closed in H12. eauto. econstructor.
           eapply index_max in H7. omega. reflexivity.
         }
         destruct A as [Tx [[na A] EqTx]].
         assert (has_typed (map (substt x) [T1x]) G1 (subst_tm x tx) (substt x (open 0 (TVar false 1) T2x))) as HIx.
-        eapply hastp_subst_z. eapply H13. rewrite EqTx. eapply A.
+        eapply hastp_subst_z. eapply H19. rewrite EqTx. eapply A.
         eu. simpl in HIx.
         assert (has_typed (map (substt x0) []) G1
                           (subst_tm x0 (subst_tm x tx))
                           (substt x0 (substt x (open 0 (TVar false 1) T2x)))) as HIx0. {
           eapply hastp_subst. rewrite app_nil_l. eapply HIx.
-          simpl in H11. inversion H11. unfold substt. rewrite H9. eauto.
+          rewrite <- HeqT0. eauto.
         }
         eu. simpl in HIx0.
         assert ((substt x (open 0 (TVar false 1) T2x))=(open 0 (TVar false 0) (substt x T2x))) as EqT2x. {
           change 1 with (0+1). rewrite subst_open. reflexivity.
         }
         assert (has_typed [] G1 (subst_tm x0 t) (substt x0 (open 0 (TVar false 0) T2))) as HI. {
-          inversion H11; subst. unfold substt in EqT2x. rewrite <- EqT2x. eauto.
+          inversion H13; subst. rewrite <- EqT2x. eexists. eapply HIx0.
         }
         eu. simpl in HI.
-        edestruct stp_subst_narrow as [? HI2]. rewrite app_nil_l. eapply H23. eauto.
+        edestruct stp_subst_narrow as [? HI2]. rewrite app_nil_l. eapply H29. eauto.
         simpl in HI2.
         assert (substt x0 (open 0 (TVar false 0) T) = T) as EqT. {
           erewrite <- closed_no_open. erewrite subst_closed_id. reflexivity.
@@ -1019,32 +1031,33 @@ Proof.
       assert (exists m n1, vtp m G1 x (TFun l T1 T2) n1). eapply hastp_inv. eauto.
       assert (exists m n1, vtp m G1 x2 T1 n1). eapply hastp_inv. eauto.
       ev. inversion H1. subst.
+      remember (substt x T1x) as T0. remember (substt x T2x) as T3.
       assert (vtpdd x0 G1 x2 T0). eapply vtp_widen. eauto. eauto. eauto. eauto. eauto.
       euv.
       assert (exists T, (exists n1, has_type [] G1 (tvar true x) T n1) /\ substt x T' = T) as A. {
         eexists. split. eexists. eapply T_Vary. eauto. eauto. eauto. eauto.
-        eapply closed_subst. eapply dms_has_type_closed in H10. eauto. econstructor.
+        eapply closed_subst. eapply dms_has_type_closed in H12. eauto. econstructor.
         eapply index_max in H7. omega. reflexivity.
       }
       destruct A as [Tx [[na A] EqTx]].
       assert (has_typed (map (substt x) [T1x]) G1 (subst_tm x tx) (substt x (open 0 (TVar false 1) T2x))) as HIx.
-      eapply hastp_subst_z. eapply H13. rewrite EqTx. eapply A.
+      eapply hastp_subst_z. eapply H19. rewrite EqTx. eapply A.
       eu. simpl in HIx.
       assert (has_typed (map (substt x2) []) G1
                         (subst_tm x2 (subst_tm x tx))
                         (substt x2 (substt x (open 0 (TVar false 1) T2x)))) as HIx0. {
         eapply hastp_subst. rewrite app_nil_l. eapply HIx.
-        simpl in H11. inversion H11. unfold substt. rewrite H9. eauto.
+        rewrite <- HeqT0. eauto.
       }
       eu. simpl in HIx0.
       assert ((substt x (open 0 (TVar false 1) T2x))=(open 0 (TVar false 0) (substt x T2x))) as EqT2x. {
         change 1 with (0+1). rewrite subst_open. reflexivity.
       }
       assert (has_typed [] G1 (subst_tm x2 t) (substt x2 (open 0 (TVar false 0) T3))) as HI. {
-        inversion H11; subst. unfold substt in EqT2x. rewrite <- EqT2x. eauto.
+        inversion H13; subst. rewrite <- EqT2x. eauto.
       }
       eu. simpl in HI.
-      edestruct stp_subst_narrow as [? HI2]. rewrite app_nil_l. eapply H23. eauto.
+      edestruct stp_subst_narrow as [? HI2]. rewrite app_nil_l. eapply H29. eauto.
       simpl in HI2.
       assert ((substt x2 (open 0 (TVar false 0) T2))=(open 0 (TVar true x2) T2)) as EqT2. {
         rewrite subst_open_commute0b. erewrite subst_closed_id. reflexivity.
